noc/NoC4.v
@@ -13,33 +13,31 @@ Module MyTypeSize <: Typesize.
 End MyTypeSize.
 
 Module NoC4 := FNoc MyTypeSize.
-Import NoC4 NoC4.d.Routerfns NoC4.d.Routerfns.NOC_setup MyTypeSize.
+Import NoC4 NoC4.d.Routerfns NoC4.d.Routerfns.NOC_setup MyTypeSize. 
 
-Definition r (reg : (reg_t nocsize)) : R reg :=
+Definition r (reg : (reg_t (S nocsize))) : R reg :=
   match reg with
   |  _ => Bits.zero
   end.
 
-
-Definition sigdenote (fn : (ext_fn_t nocsize)) : Sig_denote (Sigma fn) :=
+Definition sigdenote (fn : (ext_fn_t (S nocsize))) : Sig_denote (Sigma fn) :=
   match fn with
   | _ => fun x => x +b (Bits.of_nat 9 0)
   end.
 
-Definition r_r2l (reg : (reg_t nocsize)) : R reg :=
+Definition r_r2l (reg : (reg_t (S nocsize))) : R reg :=
   match reg with
   |  _ => Bits.zero 
   end.
 
-(* Compute run_schedule r_r2l to_action sigdenote schedule. *)
 
+(* Lemma P (n:nat) (H: NoC4.d.le_t (S n) (S nocsize)) :
+  run_schedule r_r2l to_action sigdenote schedule
+    (fun ctxt =>
+      let bits_r := ctxt.[router nocsize (NoC4.d.widen_fin H (@Fin.F1 n)) state] in
+      Bits.to_nat bits_r = 0). *)
 
-(* Definition snocsize:= of_nat nocsize.
-Definition module_name:= String.to_string (String.append "NoC"%bs snocsize). *)
-(* Definition external (r: rule_name_t) := false. *)
-
-
-  Definition package :=
+Timeout 5 Definition package :=
     {|
     ip_koika :=
     {|
